Codyroux/compactness (#123)
* [DO NOT MERGE] Define a proof theory for the equational logic of magmas.

For now just soundness.

* Start adding theorems to the blueprint, clean up notation in Lean.

* Fix some rebase snafus, improve notation.

* Add a brief overview of the completness theorem.

* Nix bluprint \lean pragmas for now, to fix build.

* [FEAT] Prove compactness theorem for formal magmas.

* Remove blueprint pragmas, for now.

* Minor cleanup.

* Minor cleanup

* Fix broken proof.

* Update equational_theories.lean

* partial update of intro

---------

Co-authored-by: Pietro Monticone <38562595+pitmonticone@users.noreply.github.com>

equational_theories/FreeMagma.lean
@@ -19,6 +19,8 @@ theorem FreeMagma_op_eq_fork (α : Type u) (a b : FreeMagma α) : a ∘ b = a �
 
 notation "Lf" => FreeMagma.Leaf
 
+instance FreeMagma.Magma {α} : Magma (FreeMagma α) := ⟨ Fork ⟩
+
 def fmapFreeMagma {α : Type u} {β : Type v} (f : α → β) : FreeMagma α → FreeMagma β
   | Lf a => FreeMagma.Leaf (f a)
   | lchild ⋆ rchild => FreeMagma.Fork (fmapFreeMagma f lchild) (fmapFreeMagma f rchild)
