equational_theories/Completeness.lean
@@ -1,0 +1,213 @@
+-- Statement and proof of the completeness theorem for magmas,
+-- we roughly follow Baader & Nipkow's "Term Rewriting and All That",
+-- and
+import equational_theories.FreeMagma
+import Mathlib.Data.Set.Defs
+
+structure MagmaLaw (α : Type) where
+  lhs : FreeMagma α
+  rhs : FreeMagma α
+deriving DecidableEq
+
+local infix:60 " ≃ " => MagmaLaw.mk
+
+def substFreeMagma {α β} (t : FreeMagma α) (σ : α → FreeMagma β) : FreeMagma β :=
+match t with
+| .Leaf a => σ a
+| t₁ ⋆ t₂ => substFreeMagma t₁ σ ⋆ substFreeMagma t₂ σ
+
+infix:66 " ⬝ " => substFreeMagma
+
+@[inline, simp]
+def Ctx α := Set (MagmaLaw α)
+
+-- FIXME: figure out how to remove this.
+instance Ctx.Membership α : Membership (MagmaLaw α) (Ctx α) := ⟨ Set.instMembership.mem ⟩
+
+section DeriveDef
+
+set_option hygiene false
+
+local infix:50 " ⊢ " =>  derive
+
+-- We keep this in type, because we're going to want to gather
+-- the (finite!) set of required axioms later.
+inductive derive {α} : Ctx α → MagmaLaw α → Type :=
+| Ax Γ E (h : E ∈ Γ) : Γ ⊢ E
+| Ref Γ t : Γ ⊢ (t ≃ t)
+| Sym Γ t u : Γ ⊢ (t ≃ u) → Γ ⊢ (u ≃ t)
+| Trans Γ t u v : Γ ⊢ (t ≃ u) → Γ ⊢ (u ≃ v) → Γ ⊢ (t ≃ v)
+-- This is not as polymorphic as it could be, shouldn't be an issue at the moment
+| Subst Γ t u σ : Γ ⊢ (t ≃ u) → Γ ⊢ (t ⬝ σ ≃ u ⬝ σ)
+| Cong Γ t₁ t₂ u₁ u₂ : Γ ⊢ (t₁ ≃ t₂) → Γ ⊢ (u₁ ≃ u₂) → Γ ⊢ (t₁ ⋆ u₁ ≃ t₂ ⋆ u₂)
+
+end DeriveDef
+
+def satisfiesPhi {α G : Type} [Magma G] (φ : α → G) (E : MagmaLaw α) : Prop :=
+  evalInMagma φ E.lhs = evalInMagma φ E.rhs
+
+def satisfies {α : Type} (G : Type) [Magma G] (E : MagmaLaw α) := ∀ (φ : α → G), satisfiesPhi φ E
+
+def satisfiesSet {α : Type} (G : Type) [Magma G] (Γ : Set (MagmaLaw α)) : Prop :=
+  ∀ E ∈ Γ, satisfies G E
+
+
+def models {α} (Γ : Ctx α) (E : MagmaLaw α) : Prop :=
+  ∀ (G : Type)[Magma G], satisfiesSet G Γ → satisfies G E
+
+infix:50 " ⊧ " => (satisfies)
+
+infix:50 " ⊧ " => (satisfiesSet)
+
+infix:50 " ⊧ " => (models)
+
+infix:50 " ⊢ " => (derive)
+
+theorem SubstEval {α} G [Magma G] (t : FreeMagma α) (σ : α → FreeMagma α) (φ : α → G) :
+  evalInMagma φ (t ⬝ σ) = evalInMagma (evalInMagma φ ∘ σ) t :=
+by
+  cases t
+  case Leaf => simp [evalInMagma, substFreeMagma]
+  case Fork t₁ t₂ =>
+  simp [evalInMagma, substFreeMagma]
+  repeat rw [SubstEval]
+
+theorem Soundness {α} (Γ : Ctx α) E (h : Γ ⊢ E) : Γ ⊧ E :=
+by
+  intros G _
+  cases h
+  case Ax mem => intros mset; apply mset; trivial
+  case Ref => intros; intro; simp[satisfiesPhi]
+  -- FIXME: try aesop here, might be a 1-liner
+  case Sym t u prf =>
+    intros φ mset
+    have h := Soundness _ _ prf
+    simp [models, satisfiesPhi] at *
+    symm; apply h; trivial
+  case Trans _ _ _ prf₁ prf₂ =>
+    intros φ mset
+    have h₁ := Soundness _ _ prf₁
+    have h₂ := Soundness _ _ prf₂
+    simp [models, satisfiesPhi] at *
+    rw [h₁, h₂] <;> trivial
+  case Subst t u σ prf =>
+    intros φ mset
+    have h := Soundness _ _ prf
+    simp [models, satisfiesPhi, evalInMagma] at *
+    repeat rw [SubstEval]
+    rw [h]; trivial
+  case Cong _ _ _ prf₁ prf₂ =>
+    intros _ _
+    have h₁ := Soundness _ _ prf₁
+    have h₂ := Soundness _ _ prf₂
+    simp [models, satisfiesPhi, evalInMagma] at *
+    rw [h₁, h₂] <;> trivial
+
+-- A little trickery here: since we'd rather have the derivations in Type
+-- (we want to extract the "used" axioms, e.g.) we smush the derivation
+-- down to prop using Nonempty for creating a setoid.
+def RelOfLaws {α} (Γ : Ctx α) : FreeMagma α → FreeMagma α → Prop :=
+  λ t u ↦ Nonempty (Γ ⊢ t ≃ u)
+
+-- eazy peezy since we basically have exactly the axioms.
+theorem RelOfLaws.isEquivalence {α} (Γ : Ctx α) : Equivalence (RelOfLaws Γ) :=
+by
+  constructor <;> simp [RelOfLaws]
+  case refl =>
+    intros x; constructor; apply derive.Ref
+  case symm => intros x y h; cases h; constructor; apply derive.Sym; trivial
+  case trans =>
+    intros x y z h₁ h₂; cases h₁; cases h₂; constructor; apply derive.Trans <;> trivial
+
+instance SetoidOfLaws {α} (Γ : Ctx α): Setoid (FreeMagma α) :=
+  ⟨ RelOfLaws Γ, RelOfLaws.isEquivalence Γ ⟩
+
+
+-- This is the quotient type we care about: it will be a model of Γ.
+def FreeMagmaWithLaws {α} (Γ : Ctx α) : Type := Quotient (SetoidOfLaws Γ)
+
+@[simp]
+def embed {α} (Γ : Ctx α) (x : FreeMagma α) : FreeMagmaWithLaws Γ := Quotient.mk _ x
+
+def ForkWithLaws {α} (Γ : Ctx α) : FreeMagmaWithLaws Γ → FreeMagmaWithLaws Γ → FreeMagmaWithLaws Γ :=
+Quotient.lift₂ (λ x y ↦ embed Γ (x ⋆ y))
+(
+  by
+    simp [HasEquiv.Equiv, Setoid.r, RelOfLaws]
+    intros x z y w d₁ d₂; cases d₁; cases d₂
+    apply Quotient.sound; simp [HasEquiv.Equiv, Setoid.r, RelOfLaws]; constructor
+    apply derive.Cong <;> trivial
+)
+
+instance FreeMagmaWithLaws.Magma {α} (Γ : Ctx α) : Magma (FreeMagmaWithLaws Γ) := { op := ForkWithLaws Γ }
+
+theorem FreeMagmaWithLaws.evalInMagmaIsQuot {α} (Γ : Ctx α) (t : FreeMagma α) (σ : α → FreeMagma α):
+  evalInMagma (embed Γ ∘ σ) t = embed Γ (t ⬝ σ) :=
+by
+  cases t <;> simp [evalInMagma]
+  case Leaf => trivial
+  case Fork =>
+  simp [Magma.op, ForkWithLaws]
+  repeat rw [FreeMagmaWithLaws.evalInMagmaIsQuot]
+  simp [Quotient.lift₂, Quotient.mk, Quotient.lift]
+  apply Quot.sound; simp [Setoid.r, RelOfLaws, substFreeMagma]
+  constructor; apply derive.Ref
+
+theorem substLFId {α} (t : FreeMagma α) : t ⬝ Lf = t :=
+by
+  cases t <;> simp [substFreeMagma]
+  constructor <;> apply substLFId
+
+
+@[simp]
+def LfEmbed {α} (Γ : Ctx α) : α → FreeMagmaWithLaws Γ := embed Γ ∘ Lf
+
+-- Mostly forward reasoning here, so we delay the intros.
+theorem FreeMagmaWithLaws.isDerives {α} (Γ : Ctx α) (E : MagmaLaw α) :
+  FreeMagmaWithLaws Γ ⊧ E → Nonempty (Γ ⊢ E) :=
+by
+  simp [satisfies, satisfiesPhi, evalInMagma]
+  intros eq; have h := (eq (LfEmbed Γ))
+  simp at h
+  repeat rw [FreeMagmaWithLaws.evalInMagmaIsQuot] at h
+  have h' := Quotient.exact h
+  simp [HasEquiv.Equiv, Setoid.r, RelOfLaws] at h'
+  repeat rw [substLFId] at h'
+  apply h'
+
+-- Sadly, we falter here and use choice. Somewhat confident it's not needed.
+theorem PhiAsSubst_aux {α} (Γ : Ctx α) (φ : α → FreeMagmaWithLaws Γ) :
+  ∃ (σ : α → FreeMagma α), ∀ x, φ x = (embed Γ) (σ x) :=
+by
+  apply Classical.axiomOfChoice (r := λ x y ↦ φ x = (embed Γ) y)
+  intros x
+  have ⟨a, h⟩ := (Quotient.exists_rep (φ x))
+  exists a
+  symm; trivial
+
+theorem PhiAsSubst {α} (Γ : Ctx α) (φ : α → FreeMagmaWithLaws Γ) :
+  ∃ (σ : α → FreeMagma α), φ = (embed Γ) ∘ σ :=
+by
+  have ⟨ σ, h ⟩ := PhiAsSubst_aux Γ φ
+  exists σ
+  apply funext
+  trivial
+
+theorem FreeMagmaWithLaws.isModel {α} (Γ : Ctx α) : FreeMagmaWithLaws Γ ⊧ Γ :=
+by
+  simp [satisfiesSet]
+  intros E mem φ
+  simp [satisfiesPhi]
+  have ⟨σ, eq_sig⟩ := (PhiAsSubst _ φ)
+  rw [eq_sig]
+  repeat rw [FreeMagmaWithLaws.evalInMagmaIsQuot]
+  apply Quotient.sound; simp [HasEquiv.Equiv, Setoid.r, RelOfLaws]
+  constructor
+  apply derive.Subst; apply derive.Ax; trivial
+
+-- Birkhoff's completeness theorem
+theorem Completeness {α} (Γ : Ctx α) (E : MagmaLaw α) (h : Γ ⊧ E) : Nonempty (Γ ⊢ E) :=
+by
+  apply FreeMagmaWithLaws.isDerives
+  apply h
+  apply FreeMagmaWithLaws.isModel
